theories/iris/helpers/reduce_det/reduce_det_cvtop.v
@@ -2,11 +2,11 @@ From mathcomp Require Import ssreflect eqtype seq ssrbool.
 From stdpp Require Import base list.
 Require Export iris_reduce_det_prelude.
 
-Lemma cvtop_convert_det v v' t1 t2 sx s f s' f' es:
+Lemma cvtop_convert_det v v' t1 t2 sx s f me s' f' es:
   types_agree t1 v ->
   cvt t2 sx v = Some v' ->
-  reduce s f [AI_basic (BI_const v); AI_basic (BI_cvtop t2 CVO_convert t1 sx)] s' f' es ->
-  reduce_det_goal s f [AI_basic (BI_const v')] s' f' es [AI_basic (BI_const v); AI_basic (BI_cvtop t2 CVO_convert t1 sx)].
+  reduce s f [AI_basic (BI_const v); AI_basic (BI_cvtop t2 CVO_convert t1 sx)] me s' f' es ->
+  reduce_det_goal ME_empty s f [AI_basic (BI_const v')] me s' f' es [AI_basic (BI_const v); AI_basic (BI_cvtop t2 CVO_convert t1 sx)].
 Proof.
   move => H H0 Hred.
   by only_one [AI_basic (BI_const v) ; AI_basic (BI_cvtop t2 CVO_convert t1 sx)] Hred ;
@@ -14,11 +14,11 @@ Proof.
      inversion H2 ; subst.
 Qed.
 
-Lemma cvtop_convert_none_det v t1 t2 sx s f s' f' es:
+Lemma cvtop_convert_none_det v t1 t2 sx s f me s' f' es:
   types_agree t1 v ->
   cvt t2 sx v = None ->
-  reduce s f [AI_basic (BI_const v); AI_basic (BI_cvtop t2 CVO_convert t1 sx)] s' f' es ->
-  reduce_det_goal s f [AI_trap] s' f' es [AI_basic (BI_const v); AI_basic (BI_cvtop t2 CVO_convert t1 sx)].
+  reduce s f [AI_basic (BI_const v); AI_basic (BI_cvtop t2 CVO_convert t1 sx)] me s' f' es ->
+  reduce_det_goal ME_empty s f [AI_trap] me s' f' es [AI_basic (BI_const v); AI_basic (BI_cvtop t2 CVO_convert t1 sx)].
 Proof.
   move => H H0 Hred.
   by only_one [AI_basic (BI_const v) ; AI_basic (BI_cvtop t2 CVO_convert t1 sx)] Hred ;
@@ -26,10 +26,10 @@ Proof.
      inversion H2 ; subst.
 Qed.
 
-Lemma cvtop_reinterpret_det v t1 t2 s f s' f' es:
+Lemma cvtop_reinterpret_det v t1 t2 s f me s' f' es:
   types_agree t1 v ->
-  reduce s f [AI_basic (BI_const v); AI_basic (BI_cvtop t2 CVO_reinterpret t1 None)] s' f' es ->
-  reduce_det_goal s f [AI_basic (BI_const (wasm_deserialise (bits v) t2))] s' f' es
+  reduce s f [AI_basic (BI_const v); AI_basic (BI_cvtop t2 CVO_reinterpret t1 None)] me s' f' es ->
+  reduce_det_goal ME_empty s f [AI_basic (BI_const (wasm_deserialise (bits v) t2))] me s' f' es
     [AI_basic (BI_const v); AI_basic (BI_cvtop t2 CVO_reinterpret t1 None)].
 Proof.
   move => H Hred.
