theories/iris/helpers/reduce_det/reduce_det_relop.v
@@ -2,9 +2,9 @@ From mathcomp Require Import ssreflect eqtype seq ssrbool.
 From stdpp Require Import base list.
 Require Export iris_reduce_det_prelude.
 
-Lemma relop_det v1 v2 op t s f s' f' es:
-  reduce s f [AI_basic (BI_const v1); AI_basic (BI_const v2); AI_basic (BI_relop t op)] s' f' es ->
-  reduce_det_goal s f [AI_basic (BI_const (VAL_int32 (wasm_bool (app_relop op v1 v2))))] s' f' es [AI_basic (BI_const v1); AI_basic (BI_const v2); AI_basic (BI_relop t op)].
+Lemma relop_det v1 v2 op t s f me s' f' es:
+  reduce s f [AI_basic (BI_const v1); AI_basic (BI_const v2); AI_basic (BI_relop t op)] me s' f' es ->
+  reduce_det_goal ME_empty s f [AI_basic (BI_const (VAL_int32 (wasm_bool (app_relop op v1 v2))))] me s' f' es [AI_basic (BI_const v1); AI_basic (BI_const v2); AI_basic (BI_relop t op)].
 Proof.
   move => Hred.
   by only_one [AI_basic (BI_const v1) ; AI_basic (BI_const v2) ; AI_basic (BI_relop t op)] Hred.
