theories/iris/helpers/reduce_det/reduce_det_select.v
@@ -2,10 +2,10 @@ From mathcomp Require Import ssreflect eqtype seq ssrbool.
 From stdpp Require Import base list.
 Require Export iris_reduce_det_prelude.
 
-Lemma select_false_det v1 v2 n s f s' f' es:
+Lemma select_false_det v1 v2 n s f me s' f' es:
   n = Wasm_int.int_zero i32m ->
-  reduce s f [AI_basic (BI_const v1); AI_basic (BI_const v2); AI_basic (BI_const (VAL_int32 n)); AI_basic BI_select] s' f' es ->
-  reduce_det_goal s f [AI_basic (BI_const v2)] s' f' es [AI_basic (BI_const v1); AI_basic (BI_const v2); AI_basic (BI_const (VAL_int32 n)); AI_basic BI_select].
+  reduce s f [AI_basic (BI_const v1); AI_basic (BI_const v2); AI_basic (BI_const (VAL_int32 n)); AI_basic BI_select] me s' f' es ->
+  reduce_det_goal ME_empty s f [AI_basic (BI_const v2)] me s' f' es [AI_basic (BI_const v1); AI_basic (BI_const v2); AI_basic (BI_const (VAL_int32 n)); AI_basic BI_select].
 Proof.
   move => H Hred.
   only_one [AI_basic (BI_const v1) ; AI_basic (BI_const v2);
@@ -13,10 +13,10 @@ Proof.
     [done | by inversion Heqes ; subst ].
 Qed.
 
-Lemma select_true_det v1 v2 n s f s' f' es:
+Lemma select_true_det v1 v2 n s f me s' f' es:
   n <> Wasm_int.int_zero i32m ->
-  reduce s f [AI_basic (BI_const v1); AI_basic (BI_const v2); AI_basic (BI_const (VAL_int32 n)); AI_basic BI_select] s' f' es ->
-  reduce_det_goal s f [AI_basic (BI_const v1)] s' f' es [AI_basic (BI_const v1); AI_basic (BI_const v2); AI_basic (BI_const (VAL_int32 n)); AI_basic BI_select].
+  reduce s f [AI_basic (BI_const v1); AI_basic (BI_const v2); AI_basic (BI_const (VAL_int32 n)); AI_basic BI_select] me s' f' es ->
+  reduce_det_goal ME_empty s f [AI_basic (BI_const v1)] me s' f' es [AI_basic (BI_const v1); AI_basic (BI_const v2); AI_basic (BI_const (VAL_int32 n)); AI_basic BI_select].
 Proof.
   move => H Hred.
   only_one [AI_basic (BI_const v1) ; AI_basic (BI_const v2);
